src/BinEncoders/Env/Common/Compose.v
@@ -3,35 +3,41 @@ Require Import
 
 Set Implicit Arguments.
 
-Definition compose E
-           (transformer : Transformer)
-           (encode1 : E -> bin * E)
-           (encode2 : E -> bin * E) :=
+Definition compose E B
+           (transformer : Transformer B)
+           (encode1 : E -> B * E)
+           (encode2 : E -> B * E) :=
   fun e0 =>
     let (p, e1) := encode1 e0 in
     let (q, e2) := encode2 e1 in
     (transform p q, e2).
 
+Notation "x 'Then' y" := (compose _ x y) (at level 100, right associativity).
+Notation "x 'Done'"   := (x Then fun e => (nil, e)) (at level 99, right associativity).
 
-Lemma compose_decoder_correct A A'
+Lemma compose_encode_correct A A' B
       (cache : Cache)
-      (transformer : Transformer)
+      (transformer : Transformer B)
       (project : A -> A')
       (predicate : A -> Prop)
       (predicate' : A' -> Prop)
-      (encode1 : A' -> CacheEncode -> bin * CacheEncode)
-      (encode2 : A -> CacheEncode -> bin * CacheEncode)
-      (decoder1 : decoder cache transformer predicate' encode1)
+      (encode1 : A' -> CacheEncode -> B * CacheEncode)
+      (encode2 : A -> CacheEncode -> B * CacheEncode)
+      (decode1 : B -> CacheDecode -> A' * B * CacheDecode)
+      (decode1_pf : encode_decode_correct cache transformer predicate' encode1 decode1)
       (pred_pf : forall data, predicate data -> predicate' (project data))
-      (decoder2 : forall proj,
-          decoder cache transformer (fun data => predicate data /\ project data = proj) encode2)
+      (decode2 : A' -> B -> CacheDecode -> A * B * CacheDecode)
+      (decode2_pf : forall proj,
+          encode_decode_correct cache transformer
+            (fun data => predicate data /\ project data = proj)
+            encode2
+            (decode2 proj))
   : encode_decode_correct cache transformer predicate
      (fun (data : A) (ctx : CacheEncode) =>
       compose transformer (encode1 (project data)) (encode2 data) ctx)
-     (fun (bin : bin) (env : CacheDecode) =>
-      let (bundle, env') := decode (decoder:=decoder1) bin env in let (proj, rest) := bundle in decode (decoder:=decoder2 proj) rest env').
+     (fun (bin : B) (env : CacheDecode) =>
+      let (bundle, env') := decode1 bin env in let (proj, rest) := bundle in decode2 proj rest env').
 Proof.
-  destruct decoder1 as [decode1 decode1_pf]. simpl.
   intros env env' xenv xenv' data data' bin ext ext' env_pm pred_pm com_pf.
   unfold compose in com_pf.
   destruct (encode1 (project data) env) as [b1 e1] eqn: eq1.
@@ -40,29 +46,7 @@ Proof.
   destruct (decode1_pf _ _ _ _ _ _ _ _ _ env_pm (pred_pf _ pred_pm) eq1 eq1') as [de [dp dt]].
   inversion com_pf; subst; clear com_pf.
   rewrite <- transform_assoc. rewrite eq1'.
-  destruct (decoder2 (project data)) as [decode2 decode2_pf]. simpl.
-  destruct (decode2 (transform b2 ext) e1') as [[d2 r2] e2'] eqn: eq2'.
-  specialize (decode2_pf _ _ _ _ _ _ _ _ _ de (conj pred_pm eq_refl) eq2 eq2').
+  destruct (decode2 (project data) (transform b2 ext) e1') as [[d2 r2] e2'] eqn: eq2'.
+  specialize (decode2_pf (project data)  _ _ _ _ _ _ _ _ _ de (conj pred_pm eq_refl) eq2 eq2').
   inversion 1. subst. intuition.
 Qed.
-
-Global Instance compose_decoder A A'
-       (cache : Cache)
-       (transformer : Transformer)
-       (project : A -> A')
-       (predicate : A -> Prop)
-       (predicate' : A' -> Prop)
-       (encode1 : A' -> CacheEncode -> bin * CacheEncode)
-       (encode2 : A -> CacheEncode -> bin * CacheEncode)
-       (decoder1 : decoder cache transformer predicate' encode1)
-       (pred_pf : forall data, predicate data -> predicate' (project data))
-       (decoder2 : forall proj,
-           decoder cache transformer (fun data => predicate data /\ project data = proj) encode2)
-  : decoder cache transformer predicate
-            (fun data ctx => compose transformer (encode1 (project data)) (encode2 data) ctx) :=
-  { decode := fun bin env => let (bundle, env') := @decode _ _ _ _ _ decoder1 bin env in
-                             let (proj, rest) := bundle in
-                             @decode _ _ _ _ _ (decoder2 proj) rest env' }.
-Proof.
-  apply compose_decoder_correct. eauto.
-Defined.
