src/BinEncoders/Env/Common/Specs.v
@@ -7,13 +7,14 @@ Set Implicit Arguments.
 
 Section Specifications.
   Variable A : Type.
+  Variable B : Type.
 
   Definition encode_decode_correct
              (cache : Cache)
-             (transformer : Transformer)
+             (transformer : Transformer B)
              (predicate : A -> Prop)
-             (encode : A -> CacheEncode -> bin * CacheEncode)
-             (decode :  bin -> CacheDecode -> A * bin * CacheDecode) :=
+             (encode : A -> CacheEncode -> B * CacheEncode)
+             (decode : B -> CacheDecode -> A * B * CacheDecode) :=
     forall env env' xenv xenv' data data' bin ext ext',
       Equiv env env' ->
       predicate data ->
@@ -21,11 +22,15 @@ Section Specifications.
       decode (transform bin ext) env' = (data', ext', xenv') ->
       Equiv xenv xenv' /\ data = data' /\ ext = ext'.
 
-  Class decoder
-        (cache : Cache)
-        (transformer : Transformer)
-        (predicate : A -> Prop)
-        (encode : A -> CacheEncode -> bin * CacheEncode) :=
-    { decode : bin -> CacheDecode -> A * bin * CacheDecode;
-      decode_correct : encode_decode_correct cache transformer predicate encode decode }.
+  (* Definition encode_decode_correct_deep
+             (cache : Cache)
+             (transformer : Transformer)
+             (predicate : A -> Prop)
+             (encode : A -> CacheEncode -> bin * CacheEncode)
+             (decode :  bin -> CacheDecode -> option (A * bin * CacheDecode)) :=
+    forall env env' xenv xenv' data data' bin ext ext',
+      Equiv env env' ->
+      predicate data ->
+      encode data env = (bin, xenv) ->
+      (decode (transform bin ext) env' = Some (data', ext', xenv') <-> Equiv xenv xenv' /\ data = data' /\ ext = ext'). *)
 End Specifications.
