src/BinEncoders/Env/Common/Transformer.v
@@ -1,8 +1,7 @@
 Set Implicit Arguments.
 
-Class Transformer :=
-  { bin : Type;
-    transform : bin -> bin -> bin;
+Class Transformer (bin : Type) :=
+  { transform : bin -> bin -> bin;
     transform_id : bin;
     transform_id_left : forall l, transform transform_id l = l;
     transform_id_right : forall l, transform l transform_id = l;
