src/BinEncoders/Env/Examples/Dns.v
@@ -1,12 +1,10 @@
 Require Import
         Fiat.BinEncoders.Env.Examples.DnsMap.
-
 Require Import
         Fiat.BinEncoders.Env.Common.Specs
         Fiat.BinEncoders.Env.Common.Sig
         Fiat.BinEncoders.Env.Common.Compose
         Fiat.BinEncoders.Env.Automation.Solver.
-
 Require Import
         Fiat.BinEncoders.Env.BinLib.Core
         Fiat.BinEncoders.Env.BinLib.FixInt
@@ -19,112 +17,125 @@ Require Import
 
 Set Implicit Arguments.
 
-Notation compose := Fiat.BinEncoders.Env.Common.Compose.compose.
-Notation "x 'Then' y" := (compose btransformer x y) (at level 100, right associativity).
-Notation "x 'Done'"   := (x Then fun e => (nil, e)) (at level 99, right associativity).
-Notation "[ n ]" := (exist _ n _).
+Section DnsExample.
+  Context {cache : Cache}.
+  Context {cacheAddN : CacheAdd cache N}.
+  Context {cacheAddPair : CacheAdd cache (list word_t * position_t)}.
+  Context {cachePeek : CachePeek cache position_t}.
+  Context {cacheGet : CacheGet cache (list word_t) position_t}.
 
-Inductive type_t := A | CNAME | NS | MX.
-Inductive class_t := IN | CH | HS.
+  Inductive type_t := A | CNAME | NS | MX.
+  Inductive class_t := IN | CH | HS.
 
-Definition halt : word_t.
-  refine (Build_word_t (exist _ nil _));
-    abstract (rewrite Compare_dec.nat_compare_lt; eauto). Defined.
-Definition halt_dec (a : word_t) : {a = halt} + {a <> halt}.
-  unfold halt; destruct a as [[word word_pf]];
-  destruct word eqn: eq; subst.
-  - left; abstract (f_equal; apply sig_equivalence; eauto).
-  - right; abstract (inversion 1).
-Defined. Hint Resolve halt_dec.
+  Definition halt : word_t.
+    refine (Build_word_t (exist _ nil _));
+      abstract (rewrite Compare_dec.nat_compare_lt; eauto). Defined.
 
-Record name_t :=
-  { name : { s : list word_t | length s <= 255 /\ forall x, In x s -> x <> halt } }.
+  Definition halt_dec (a : word_t) : {a = halt} + {a <> halt}.
+    unfold halt; destruct a as [[word word_pf]];
+      destruct word eqn: eq; subst.
+    - left; abstract (f_equal; apply sig_equivalence; eauto).
+    - right; abstract (inversion 1).
+  Defined. Hint Resolve halt_dec.
 
-Record question_t :=
-  { qname  : name_t;
-    qtype  : type_t;
-    qclass : class_t }.
+  Record name_t :=
+    { name : { s : list word_t | length s <= 255 /\ forall x, In x s -> x <> halt } }.
 
-Record resource_t :=
-  { rname  : name_t;
-    rtype  : type_t;
-    rclass : class_t;
-    rttl   : uint 32;
-    rdata  : { s : list ascii |  length s < exp2_nat 16 } }.
+  Record question_t :=
+    { qname  : name_t;
+      qtype  : type_t;
+      qclass : class_t }.
 
-Record packet_t :=
-  { pid         : { s : list bool | length s = 16 };
-    pmask       : { s : list bool | length s = 16 };
-    pquestion   : { s : list question_t | length s < exp2_nat 16 };
-    panswer     : { s : list resource_t | length s < exp2_nat 16 };
-    pauthority  : { s : list resource_t | length s < exp2_nat 16 };
-    padditional : { s : list resource_t | length s < exp2_nat 16 } }.
+  Record resource_t :=
+    { rname  : name_t;
+      rtype  : type_t;
+      rclass : class_t;
+      rttl   : uint 32;
+      rdata  : { s : list ascii |  length s < exp2_nat 16 } }.
 
-Definition FixInt_of_branch (b : CacheBranch) : {n | (n < exp2 2)%N}.
-  refine (match b with
-          | Yes => [3%N]
-          | No  => [0%N]
-          end); abstract (rewrite <- N.compare_lt_iff; eauto).  Defined.
+  Record packet_t :=
+    { pid         : { s : list bool | length s = 16 };
+      pmask       : { s : list bool | length s = 16 };
+      pquestion   : { s : list question_t | length s < exp2_nat 16 };
+      panswer     : { s : list resource_t | length s < exp2_nat 16 };
+      pauthority  : { s : list resource_t | length s < exp2_nat 16 };
+      padditional : { s : list resource_t | length s < exp2_nat 16 } }.
 
-Definition FixInt_of_type (t : type_t) : {n | (n < exp2 16)%N}.
-  refine (match t with
-          | A     => [1%N]
-          | CNAME => [5%N]
-          | NS    => [2%N]
-          | MX    => [15%N]
-          end); abstract (rewrite <- N.compare_lt_iff; eauto).  Defined.
+  Definition FixInt_of_branch (b : CacheBranch) : {n | (n < exp2 2)%N}.
+    refine (match b with
+            | Yes => [3%N]
+            | No  => [0%N]
+            end); abstract (rewrite <- N.compare_lt_iff; eauto).  Defined.
 
-Definition FixInt_of_class (c : class_t) : {n | (n < exp2 16)%N}.
-  refine (match c with
-          | IN => [1%N]
-          | CH => [3%N]
-          | HS => [4%N]
-          end); abstract (rewrite <- N.compare_lt_iff; eauto).  Defined.
+  Definition FixInt_of_type (t : type_t) : {n | (n < exp2 16)%N}.
+    refine (match t with
+            | A     => [1%N]
+            | CNAME => [5%N]
+            | NS    => [2%N]
+            | MX    => [15%N]
+            end); abstract (rewrite <- N.compare_lt_iff; eauto).  Defined.
 
-Definition encode_word (w : word_t) :=
-       FixInt_encode (FixList_getlength w.(word))
-  Then FixList_encode btransformer Char_encode w.(word)
-  Done.
+  Definition FixInt_of_class (c : class_t) : {n | (n < exp2 16)%N}.
+    refine (match c with
+            | IN => [1%N]
+            | CH => [3%N]
+            | HS => [4%N]
+            end); abstract (rewrite <- N.compare_lt_iff; eauto).  Defined.
 
-Definition encode_name (n : name_t) :=
-       SteppingList_encode btransformer encode_word FixInt_encode
-                           (Enum_encode FixInt_of_branch) n.(name)
-  Done.
+  Definition encode_word (w : word_t) :=
+         FixInt_encode (FixList_getlength w.(word))
+    Then FixList_encode Char_encode w.(word)
+    Done.
 
-Definition encode_question (q : question_t) :=
-       encode_name q.(qname)
-  Then Enum_encode FixInt_of_type q.(qtype)
-  Then Enum_encode FixInt_of_class q.(qclass)
-  Done.
+  Definition encode_name (n : name_t) :=
+         SteppingList_encode encode_word FixInt_encode (Enum_encode FixInt_of_branch) n.(name)
+    Done.
 
-Definition encode_resource (r : resource_t) :=
-       encode_name r.(rname)
-  Then Enum_encode FixInt_of_type r.(rtype)
-  Then Enum_encode FixInt_of_class r.(rclass)
-  Then FixInt_encode r.(rttl)
-  Then FixInt_encode (FixList_getlength r.(rdata))
-  Then FixList_encode btransformer Char_encode r.(rdata)
-  Done.
+  Definition encode_question (q : question_t) :=
+         encode_name q.(qname)
+    Then Enum_encode FixInt_of_type q.(qtype)
+    Then Enum_encode FixInt_of_class q.(qclass)
+    Done.
 
-Definition encode_packet (p : packet_t) :=
-       IList_encode btransformer Bool_encode p.(pid)
-  Then IList_encode btransformer Bool_encode p.(pmask)
-  Then FixInt_encode (FixList_getlength p.(pquestion))
-  Then FixInt_encode (FixList_getlength p.(panswer))
-  Then FixInt_encode (FixList_getlength p.(pauthority))
-  Then FixInt_encode (FixList_getlength p.(padditional))
-  Then FixList_encode btransformer encode_question p.(pquestion)
-  Then FixList_encode btransformer encode_resource p.(panswer)
-  Then FixList_encode btransformer encode_resource p.(pauthority)
-  Then FixList_encode btransformer encode_resource p.(padditional)
-  Done.
+  Definition encode_resource (r : resource_t) :=
+         encode_name r.(rname)
+    Then Enum_encode FixInt_of_type r.(rtype)
+    Then Enum_encode FixInt_of_class r.(rclass)
+    Then FixInt_encode r.(rttl)
+    Then FixInt_encode (FixList_getlength r.(rdata))
+    Then FixList_encode Char_encode r.(rdata)
+    Done.
 
+  Definition encode_packet (p : packet_t) :=
+         IList_encode Bool_encode p.(pid)
+    Then IList_encode Bool_encode p.(pmask)
+    Then FixInt_encode (FixList_getlength p.(pquestion))
+    Then FixInt_encode (FixList_getlength p.(panswer))
+    Then FixInt_encode (FixList_getlength p.(pauthority))
+    Then FixInt_encode (FixList_getlength p.(padditional))
+    Then FixList_encode encode_question p.(pquestion)
+    Then FixList_encode encode_resource p.(panswer)
+    Then FixList_encode encode_resource p.(pauthority)
+    Then FixList_encode encode_resource p.(padditional)
+    Done.
 
-Global Instance packet_decoder
-  : decoder cache btransformer (fun _ => True) encode_packet.
-Proof.
-  Time solve_decoder. (* now works in 8.4pl6 -- takes about 10 seconds. *)
-Defined.
+  Definition packet_decoder
+    : { decode | encode_decode_correct cache btransformer (fun _ => True) encode_packet decode }.
+  Proof.
+    eexists.
+    Time solve_decoder.
+    Grab Existential Variables.
+    eauto. eauto. eauto. eauto.
+  Defined.
+
+  Definition packet_decoder'
+    : list bool -> CacheDecode -> packet_t * list bool * CacheDecode.
+  Proof.
+    let p' := eval cbv delta [ proj1_sig packet_decoder ] beta iota in (proj1_sig packet_decoder) in
+                                                                        pose p' as p.
+    exact p.
+  Defined.
+End DnsExample.
 
 Definition empty :=
   {| eMap := EMap.empty _;
@@ -141,35 +152,36 @@ Definition packet_encode (p : packet_t) : list bool :=
   fst (encode_packet p empty).
 
 Definition packet_decode (b : list bool) : packet_t :=
-  fst (fst (decode (decoder:=packet_decoder) b empty)).
+  fst (fst (packet_decoder' b empty)).
 
 Theorem this_is_correct_and_we_know_it :
   forall p, packet_decode (packet_encode p) = p.
 Proof.
   intro p.
   unfold packet_encode, packet_decode.
-  pose proof (@decode_correct _ cache btransformer _ _ packet_decoder empty empty
-                (snd (encode_packet p empty))
-                (snd (decode (transform (fst (encode_packet p empty)) transform_id) empty))
-                p
-                (fst (fst (decode (transform (fst (encode_packet p empty)) transform_id) empty)))
-                (fst (encode_packet p empty))
-                transform_id
-                (snd (fst (decode (transform (fst (encode_packet p empty)) transform_id) empty)))
-                empty_Equiv
-                I).
-  destruct (encode_packet p empty).
+  pose proof (proj2_sig packet_decoder empty empty
+    (snd (encode_packet p empty))
+    (snd (packet_decoder' (transform (fst (encode_packet p empty)) transform_id) empty))
+    p
+    (fst (fst (packet_decoder' (transform (fst (encode_packet p empty)) transform_id) empty)))
+    (fst (encode_packet p empty))
+    transform_id
+    (snd (fst (packet_decoder' (transform (fst (encode_packet p empty)) transform_id) empty)))
+    empty_Equiv
+    I).
+  destruct (@encode_packet cache cacheAddN cacheAddPair cachePeek cacheGet p empty).
   rewrite transform_id_right in H.
-  destruct (decode (decoder:=packet_decoder) (fst (b, c)) empty) as [[? ?] ?].
+  change (proj1_sig packet_decoder) with packet_decoder' in H.
+  destruct (@packet_decoder' cache cacheAddN cacheAddPair cachePeek cacheGet
+           (fst (l, c)) empty) as [[? ?] ?].
   specialize (H eq_refl eq_refl).
-  intuition.  Qed.
+  intuition.
+Qed.
 
-Section Examples.
-  Definition packet_uncompressed :=
-    true :: true :: false :: true :: true :: false :: true :: true :: false :: true :: false :: false :: false :: false :: true :: false :: false :: false :: false :: false :: false :: false :: false :: true :: false :: false :: false :: false :: false :: false :: false :: false :: false :: false :: false :: false :: false :: false :: false :: false :: false :: false :: false :: false :: false :: false :: false :: true :: false :: false :: false :: false :: false :: false :: false :: false :: false :: false :: false :: false :: false :: false :: false :: false :: false :: false :: false :: false :: false :: false :: false :: false :: false :: false :: false :: false :: false :: false :: false :: false :: false :: false :: false :: false :: false :: false :: false :: false :: false :: false :: false :: false :: false :: false :: false :: false :: false :: false :: false :: false :: false :: false :: true :: true :: false :: true :: true :: true :: false :: true :: true :: true :: false :: true :: true :: true :: false :: true :: true :: true :: false :: true :: true :: true :: false :: true :: true :: true :: false :: false :: false :: false :: true :: true :: false :: false :: false :: true :: true :: false :: true :: true :: true :: false :: false :: true :: true :: false :: true :: true :: true :: true :: false :: true :: true :: true :: false :: false :: true :: false :: false :: true :: true :: true :: false :: true :: false :: false :: false :: true :: true :: false :: true :: false :: false :: false :: false :: true :: true :: false :: false :: true :: false :: true :: false :: true :: true :: false :: false :: false :: false :: true :: false :: true :: true :: true :: false :: false :: true :: true :: false :: true :: true :: true :: false :: true :: false :: false :: false :: true :: true :: false :: false :: true :: false :: true :: false :: true :: true :: true :: false :: false :: true :: false :: false :: true :: true :: false :: true :: true :: true :: false :: false :: false :: false :: false :: false :: false :: true :: true :: false :: true :: true :: false :: false :: true :: false :: true :: false :: true :: true :: false :: false :: true :: false :: false :: false :: true :: true :: true :: false :: true :: false :: true :: false :: false :: false :: false :: false :: false :: false :: false :: false :: false :: false :: false :: false :: false :: false :: false :: false :: false :: false :: false :: false :: false :: false :: true :: false :: false :: false :: false :: false :: false :: false :: false :: false :: false :: false :: false :: false :: false :: false :: true :: nil.
-  Definition packet_compressed :=
-    true :: true :: false :: true :: true :: false :: true :: true :: false :: true :: false :: false :: false :: false :: true :: false :: true :: false :: false :: false :: false :: false :: false :: true :: true :: false :: false :: false :: false :: false :: false :: false :: false :: false :: false :: false :: false :: false :: false :: false :: false :: false :: false :: false :: false :: false :: false :: true :: false :: false :: false :: false :: false :: false :: false :: false :: false :: false :: false :: false :: false :: false :: false :: true :: false :: false :: false :: false :: false :: false :: false :: false :: false :: false :: false :: false :: false :: false :: false :: false :: false :: false :: false :: false :: false :: false :: false :: false :: false :: false :: false :: false :: false :: false :: false :: false :: false :: false :: false :: false :: false :: false :: true :: true :: false :: true :: true :: true :: false :: true :: true :: true :: false :: true :: true :: true :: false :: true :: true :: true :: false :: true :: true :: true :: false :: true :: true :: true :: false :: false :: false :: false :: true :: true :: false :: false :: false :: true :: true :: false :: true :: true :: true :: false :: false :: true :: true :: false :: true :: true :: true :: true :: false :: true :: true :: true :: false :: false :: true :: false :: false :: true :: true :: true :: false :: true :: false :: false :: false :: true :: true :: false :: true :: false :: false :: false :: false :: true :: true :: false :: false :: true :: false :: true :: false :: true :: true :: false :: false :: false :: false :: true :: false :: true :: true :: true :: false :: false :: true :: true :: false :: true :: true :: true :: false :: true :: false :: false :: false :: true :: true :: false :: false :: true :: false :: true :: false :: true :: true :: true :: false :: false :: true :: false :: false :: true :: true :: false :: true :: true :: true :: false :: false :: false :: false :: false :: false :: false :: true :: true :: false :: true :: true :: false :: false :: true :: false :: true :: false :: true :: true :: false :: false :: true :: false :: false :: false :: true :: true :: true :: false :: true :: false :: true :: false :: false :: false :: false :: false :: false :: false :: false :: false :: false :: false :: false :: false :: false :: false :: false :: false :: false :: false :: false :: false :: false :: false :: true :: false :: false :: false :: false :: false :: false :: false :: false :: false :: false :: false :: false :: false :: false :: false :: true :: true :: true :: false :: false :: false :: false :: false :: false :: false :: false :: false :: false :: true :: true :: false :: false :: false :: false :: false :: false :: false :: false :: false :: false :: false :: false :: false :: false :: false :: false :: false :: true :: false :: false :: false :: false :: false :: false :: false :: false :: false :: false :: false :: false :: false :: false :: false :: true :: false :: false :: false :: false :: false :: false :: false :: false :: false :: false :: false :: false :: false :: false :: false :: false :: false :: false :: false :: false :: false :: false :: true :: false :: false :: true :: false :: true :: true :: false :: false :: false :: false :: false :: false :: false :: false :: false :: false :: false :: false :: false :: false :: false :: false :: true :: false :: false :: true :: false :: false :: true :: true :: false :: true :: true :: false :: false :: true :: false :: false :: false :: false :: true :: false :: false :: false :: true :: false :: false :: false :: true :: false :: true :: false :: false :: false :: true :: false :: false :: nil.
-End Examples.
+Definition packet_uncompressed :=
+  true :: true :: false :: true :: true :: false :: true :: true :: false :: true :: false :: false :: false :: false :: true :: false :: false :: false :: false :: false :: false :: false :: false :: true :: false :: false :: false :: false :: false :: false :: false :: false :: false :: false :: false :: false :: false :: false :: false :: false :: false :: false :: false :: false :: false :: false :: false :: true :: false :: false :: false :: false :: false :: false :: false :: false :: false :: false :: false :: false :: false :: false :: false :: false :: false :: false :: false :: false :: false :: false :: false :: false :: false :: false :: false :: false :: false :: false :: false :: false :: false :: false :: false :: false :: false :: false :: false :: false :: false :: false :: false :: false :: false :: false :: false :: false :: false :: false :: false :: false :: false :: false :: true :: true :: false :: true :: true :: true :: false :: true :: true :: true :: false :: true :: true :: true :: false :: true :: true :: true :: false :: true :: true :: true :: false :: true :: true :: true :: false :: false :: false :: false :: true :: true :: false :: false :: false :: true :: true :: false :: true :: true :: true :: false :: false :: true :: true :: false :: true :: true :: true :: true :: false :: true :: true :: true :: false :: false :: true :: false :: false :: true :: true :: true :: false :: true :: false :: false :: false :: true :: true :: false :: true :: false :: false :: false :: false :: true :: true :: false :: false :: true :: false :: true :: false :: true :: true :: false :: false :: false :: false :: true :: false :: true :: true :: true :: false :: false :: true :: true :: false :: true :: true :: true :: false :: true :: false :: false :: false :: true :: true :: false :: false :: true :: false :: true :: false :: true :: true :: true :: false :: false :: true :: false :: false :: true :: true :: false :: true :: true :: true :: false :: false :: false :: false :: false :: false :: false :: true :: true :: false :: true :: true :: false :: false :: true :: false :: true :: false :: true :: true :: false :: false :: true :: false :: false :: false :: true :: true :: true :: false :: true :: false :: true :: false :: false :: false :: false :: false :: false :: false :: false :: false :: false :: false :: false :: false :: false :: false :: false :: false :: false :: false :: false :: false :: false :: false :: true :: false :: false :: false :: false :: false :: false :: false :: false :: false :: false :: false :: false :: false :: false :: false :: true :: nil.
+Definition packet_compressed :=
+  true :: true :: false :: true :: true :: false :: true :: true :: false :: true :: false :: false :: false :: false :: true :: false :: true :: false :: false :: false :: false :: false :: false :: true :: true :: false :: false :: false :: false :: false :: false :: false :: false :: false :: false :: false :: false :: false :: false :: false :: false :: false :: false :: false :: false :: false :: false :: true :: false :: false :: false :: false :: false :: false :: false :: false :: false :: false :: false :: false :: false :: false :: false :: true :: false :: false :: false :: false :: false :: false :: false :: false :: false :: false :: false :: false :: false :: false :: false :: false :: false :: false :: false :: false :: false :: false :: false :: false :: false :: false :: false :: false :: false :: false :: false :: false :: false :: false :: false :: false :: false :: false :: true :: true :: false :: true :: true :: true :: false :: true :: true :: true :: false :: true :: true :: true :: false :: true :: true :: true :: false :: true :: true :: true :: false :: true :: true :: true :: false :: false :: false :: false :: true :: true :: false :: false :: false :: true :: true :: false :: true :: true :: true :: false :: false :: true :: true :: false :: true :: true :: true :: true :: false :: true :: true :: true :: false :: false :: true :: false :: false :: true :: true :: true :: false :: true :: false :: false :: false :: true :: true :: false :: true :: false :: false :: false :: false :: true :: true :: false :: false :: true :: false :: true :: false :: true :: true :: false :: false :: false :: false :: true :: false :: true :: true :: true :: false :: false :: true :: true :: false :: true :: true :: true :: false :: true :: false :: false :: false :: true :: true :: false :: false :: true :: false :: true :: false :: true :: true :: true :: false :: false :: true :: false :: false :: true :: true :: false :: true :: true :: true :: false :: false :: false :: false :: false :: false :: false :: true :: true :: false :: true :: true :: false :: false :: true :: false :: true :: false :: true :: true :: false :: false :: true :: false :: false :: false :: true :: true :: true :: false :: true :: false :: true :: false :: false :: false :: false :: false :: false :: false :: false :: false :: false :: false :: false :: false :: false :: false :: false :: false :: false :: false :: false :: false :: false :: false :: true :: false :: false :: false :: false :: false :: false :: false :: false :: false :: false :: false :: false :: false :: false :: false :: true :: true :: true :: false :: false :: false :: false :: false :: false :: false :: false :: false :: false :: true :: true :: false :: false :: false :: false :: false :: false :: false :: false :: false :: false :: false :: false :: false :: false :: false :: false :: false :: true :: false :: false :: false :: false :: false :: false :: false :: false :: false :: false :: false :: false :: false :: false :: false :: true :: false :: false :: false :: false :: false :: false :: false :: false :: false :: false :: false :: false :: false :: false :: false :: false :: false :: false :: false :: false :: false :: false :: true :: false :: false :: true :: false :: true :: true :: false :: false :: false :: false :: false :: false :: false :: false :: false :: false :: false :: false :: false :: false :: false :: false :: true :: false :: false :: true :: false :: false :: true :: true :: false :: true :: true :: false :: false :: true :: false :: false :: false :: false :: true :: false :: false :: false :: true :: false :: false :: false :: true :: false :: true :: false :: false :: false :: true :: false :: false :: nil.
 
 Goal True.
   pose (packet_decode packet_uncompressed) as goal.
