src/BinEncoders/Env/Automation/Solver.v
@@ -48,8 +48,8 @@ Ltac solve_enum :=
   | idtac'; enum_finish ].
 
 Ltac solve_done :=
-  eexists; intros ? ? ? ? data ? ? ? ?;
-    instantiate (1:=fun b e => (_, b, e));
+  intros ? ? ? ? data ? ? ? ?;
+    instantiate (1:=fun _ b e => (_, b, e));
     intros; destruct data; simpl in *; repeat match goal with
                    | H : (_, _) = (_, _) |- _ => inversion H; subst; clear H
                    | H : _ /\ _ |- _ => inversion H; subst; clear H
@@ -61,18 +61,18 @@ Ltac solve_predicate :=
 
 Ltac eauto_typeclass :=
   match goal with
-  | |- context [ Bool_encode ] => eapply Bool_decoder
-  | |- context [ Char_encode ] => eapply Char_decoder
-  | |- context [ FixInt_encode ] => eapply FixInt_decoder
-  | |- context [ FixList_encode _ _ ] => eapply FixList_decoder
-  | |- context [ IList_encode _ _ ] => eapply IList_decoder
-  | |- context [ SteppingList_encode _ _ _ _ ] => eapply SteppingListCache_decoder
+  | |- context [ Bool_encode ] => eapply Bool_encode_correct
+  | |- context [ Char_encode ] => eapply Char_encode_correct
+  | |- context [ FixInt_encode ] => eapply FixInt_encode_correct
+  | |- context [ FixList_encode _ ] => eapply FixList_encode_correct
+  | |- context [ IList_encode _ ] => eapply IList_encode_correct
+  | |- context [ SteppingList_encode _ _ _ ] => eapply SteppingList_encode_correct
   end; eauto.
 
 Ltac solve_decoder :=
   match goal with
   | |- _ => solve [ eauto_typeclass; solve_decoder ]
-  | |- _ => solve [ eapply Enum_decoder; solve_enum ]
+  | |- _ => solve [ eapply Enum_encode_correct; solve_enum ]
   | |- _ => solve [ solve_done ]
-  | |- _ => eapply compose_decoder; [ solve_decoder | solve_predicate | intro; solve_decoder ]
+  | |- _ => eapply compose_encode_correct; [ solve_decoder | solve_predicate | intro; solve_decoder ]
   end.
