src/BinEncoders/Env/BinLib/FixInt.v
@@ -253,9 +253,4 @@ Section FixIntBinEncoder.
   Qed.
 End FixIntBinEncoder.
 
-Global Instance FixInt_decoder size cache cacheAdd predicate
-  : decoder cache btransformer predicate (@FixInt_encode size cache cacheAdd) :=
-  { decode := @FixInt_decode size cache cacheAdd;
-    decode_correct := @FixInt_encode_correct _ _ _ _ }.
-
 Arguments FixInt_encode {_ _ _} _ _.
