src/BinEncoders/Env/Lib/SteppingCacheList.v
@@ -15,6 +15,7 @@ Inductive CacheBranch :=
 Section SteppingListCacheEncoder.
   Variable A : Type.
   Variable B : Type.
+  Variable bin : Type.
   Variable fuel : nat.
 
   Variable cache : Cache.
@@ -22,21 +23,24 @@ Section SteppingListCacheEncoder.
   Variable cacheGet : CacheGet cache (list A) B.
   Variable cachePeek : CachePeek cache B.
 
-  Variable transformer : Transformer.
+  Variable transformer : Transformer bin.
 
   Variable A_halt : A.
   Variable A_halt_dec : forall a, {a = A_halt} + {~ a = A_halt}.
   Variable A_predicate : A -> Prop.
   Variable A_encode : A -> CacheEncode -> bin * CacheEncode.
-  Variable A_decoder : decoder cache transformer A_predicate A_encode.
+  Variable A_decode : bin -> CacheDecode -> A * bin * CacheDecode.
+  Variable A_decode_pf : encode_decode_correct cache transformer A_predicate A_encode A_decode.
 
   Variable B_predicate : B -> Prop.
   Variable B_encode : B -> CacheEncode -> bin * CacheEncode.
-  Variable B_decoder : decoder cache transformer B_predicate B_encode.
+  Variable B_decode : bin -> CacheDecode -> B * bin * CacheDecode.
+  Variable B_decode_pf : encode_decode_correct cache transformer B_predicate B_encode B_decode.
 
   Variable C_predicate : CacheBranch -> Prop.
   Variable C_encode : CacheBranch -> CacheEncode -> bin * CacheEncode.
-  Variable C_decoder : decoder cache transformer C_predicate C_encode.
+  Variable C_decode : bin -> CacheDecode -> CacheBranch * bin * CacheDecode.
+  Variable C_decode_pf : encode_decode_correct cache transformer C_predicate C_encode C_decode.
 
   Definition SteppingList := { xs : list A | length xs <= fuel /\
                                              forall x, In x xs -> ~ x = A_halt }.
@@ -82,10 +86,10 @@ Section SteppingListCacheEncoder.
   Defined.
 
   Fixpoint SteppingList_decode' (f : nat) (b : bin) (cd : CacheDecode) : list A * bin * CacheDecode :=
-    let (x1, e1) := decode b cd in
+    let (x1, e1) := C_decode b cd in
     let (br, b1) := x1 in
     match br with
-    | Yes => let (x2, e2) := decode b1 e1 in
+    | Yes => let (x2, e2) := B_decode b1 e1 in
              let (ps, b2) := x2 in
              match getD cd ps with
              | Some l =>
@@ -94,7 +98,7 @@ Section SteppingListCacheEncoder.
                else (nil, b, cd) (* bogus *)
              | None => (nil, b, cd) (* bogus *)
              end
-    | No => let (x2, e2) := decode b1 e1 in
+    | No => let (x2, e2) := A_decode b1 e1 in
             let (a, b2) := x2 in
             if A_halt_dec a then
               (nil, b2, e2)
@@ -113,17 +117,17 @@ Section SteppingListCacheEncoder.
   Proof.
     generalize dependent b. generalize dependent cd.
     induction f; intros; simpl.
-    { destruct (decode b cd) as [[? ?] ?]. destruct c.
-      destruct (decode b0 c0) as [[? ?] ?]. destruct (getD cd b1).
+    { destruct (C_decode b cd) as [[? ?] ?]. destruct c.
+      destruct (B_decode b0 c0) as [[? ?] ?]. destruct (getD cd b1).
       destruct (SteppingList_ok 0 l). simpl. tauto.
       intuition. intuition.
-      destruct (decode b0 c0) as [[? ?] ?]. destruct (A_halt_dec a).
+      destruct (A_decode b0 c0) as [[? ?] ?]. destruct (A_halt_dec a).
       intuition. intuition. }
-    { destruct (decode b cd) as [[? ?] ?]. destruct c.
-      destruct (decode b0 c0) as [[? ?] ?]. destruct (getD cd b1).
+    { destruct (C_decode b cd) as [[? ?] ?]. destruct c.
+      destruct (B_decode b0 c0) as [[? ?] ?]. destruct (getD cd b1).
       destruct (SteppingList_ok (S f) l).
       intuition. intuition. intuition.
-      destruct (decode b0 c0) as [[? ?] ?].
+      destruct (A_decode b0 c0) as [[? ?] ?].
       specialize (IHf c b1).
       destruct (SteppingList_decode' f b1 c) as [[? ?] ?].
       destruct (A_halt_dec a).
@@ -143,7 +147,7 @@ Section SteppingListCacheEncoder.
     encode_decode_correct cache transformer SteppingList_predicate SteppingList_encode SteppingList_decode.
   Proof.
     unfold encode_decode_correct.
-    intros env env' xenv xenv' [l l_pf] [l' l'_pf] bin ext ext' Eeq Ppred Penc Pdec.
+    intros env env' xenv xenv' [l l_pf] [l' l'_pf] bin' ext ext' Eeq Ppred Penc Pdec.
     unfold SteppingList_predicate, SteppingList_encode, SteppingList_decode in *; simpl in *.
     inversion Pdec; subst; clear Pdec.
     rewrite <- sig_equivalence with (P:=fun xs : list A => length xs <= fuel /\ (forall x : A, In x xs -> x <> A_halt)).
@@ -151,41 +155,41 @@ Section SteppingListCacheEncoder.
 
     generalize dependent fuel; clear fuel.
     generalize dependent env; generalize dependent env';
-      generalize dependent xenv; generalize dependent bin.
+      generalize dependent xenv; generalize dependent bin'.
     induction l; intros; simpl in *.
     { destruct (C_encode No env) eqn: ?.
       destruct (A_encode A_halt c) eqn: ?.
       inversion Penc; subst; clear Penc. rewrite <- !transform_assoc.
-      destruct (decode (transform b (transform b0 ext)) env') as [[? ?] ?] eqn: ?.
-      pose proof (decode_correct (decoder:=C_decoder) env env' _ _ Eeq (H2 _) Heqp Heqp1) as [? [? ?]]. subst.
+      destruct (C_decode (transform b (transform b0 ext)) env') as [[? ?] ?] eqn: ?.
+      pose proof (C_decode_pf _ Eeq (H2 _) Heqp Heqp1) as [? [? ?]]. subst.
       destruct fuel eqn: ?; simpl; rewrite !Heqp1; clear Heqp1.
-      destruct (decode (transform b0 ext) c1) as [[? ?] ?] eqn: ?.
-      pose proof (decode_correct (decoder:=A_decoder) _ _ _ _ H3 H Heqp0 Heqp1) as [? [? ?]].
+      destruct (A_decode (transform b0 ext) c1) as [[? ?] ?] eqn: ?.
+      pose proof (A_decode_pf _ H3 H Heqp0 Heqp1) as [? [? ?]].
       rewrite <- H5. destruct (A_halt_dec A_halt). intuition. congruence.
-      destruct (decode (transform b0 ext) c1) as [[? ?] ?] eqn: ?.
-      pose proof (decode_correct (decoder:=A_decoder) _ _ _ _ H3 H Heqp0 Heqp1) as [? [? ?]].
+      destruct (A_decode (transform b0 ext) c1) as [[? ?] ?] eqn: ?.
+      pose proof (A_decode_pf _ H3 H Heqp0 Heqp1) as [? [? ?]].
       rewrite <- H5. destruct (A_halt_dec A_halt). intuition. congruence. }
     { destruct fuel as [| fuel']. exfalso. intuition.
       destruct (getE env (a :: l)) eqn: ?.
       destruct (C_encode Yes env) eqn: ?.
       destruct (B_encode b c) eqn: ?.
       inversion Penc; subst; clear Penc. rewrite <- !transform_assoc.
-      destruct (decode (transform b0 (transform b1 ext)) env') as [[? ?] ?] eqn: ?.
-      pose proof (decode_correct (decoder:=C_decoder) env env' _ _ Eeq (H2 _) Heqp Heqp1) as [? [? ?]]. subst.
+      destruct (C_decode (transform b0 (transform b1 ext)) env') as [[? ?] ?] eqn: ?.
+      pose proof (C_decode_pf _ Eeq (H2 _) Heqp Heqp1) as [? [? ?]]. subst.
       simpl. rewrite !Heqp1. clear Heqp1.
-      destruct (decode (transform b1 ext) c1) as [[? ?] ?] eqn: ?.
-      pose proof (decode_correct (decoder:=B_decoder) _ _ _ _ H3 (H1 _) Heqp0 Heqp1) as [? [? ?]]. subst.
+      destruct (B_decode (transform b1 ext) c1) as [[? ?] ?] eqn: ?.
+      pose proof (B_decode_pf _ H3 (H1 _) Heqp0 Heqp1) as [? [? ?]]. subst.
       rewrite get_correct in Heqo; eauto. rewrite !Heqo.
       destruct (SteppingList_ok (S fuel') (a :: l)); try tauto.
       destruct (C_encode No env) eqn: ?.
       destruct (A_encode a c) eqn: ?.
       destruct (SteppingList_encode' l c0) eqn: ?.
       inversion Penc; subst; clear Penc. rewrite <- !transform_assoc.
-      destruct (decode (transform b (transform b0 (transform b1 ext))) env') as [[? ?] ?] eqn: ?.
-      pose proof (decode_correct (decoder:=C_decoder) _ _ _ _ Eeq (H2 _) Heqp Heqp2) as [? [? ?]]. subst.
+      destruct (C_decode (transform b (transform b0 (transform b1 ext))) env') as [[? ?] ?] eqn: ?.
+      pose proof (C_decode_pf _ Eeq (H2 _) Heqp Heqp2) as [? [? ?]]. subst.
       simpl. rewrite !Heqp2. clear Heqp2.
-      destruct (decode (transform b0 (transform b1 ext)) c3) as [[? ?] ?] eqn: ?.
-      pose proof (decode_correct (decoder:=A_decoder) _ _ _ _ H3 (H0 a (or_introl eq_refl)) Heqp0 Heqp2) as [? [? ?]]. subst.
+      destruct (A_decode (transform b0 (transform b1 ext)) c3) as [[? ?] ?] eqn: ?.
+      pose proof (A_decode_pf _ H3 (H0 a (or_introl eq_refl)) Heqp0 Heqp2) as [? [? ?]]. subst.
       destruct (A_halt_dec a0). exfalso. subst. destruct l_pf. specialize (H6 A_halt (or_introl eq_refl)). congruence.
       assert (forall x : A, In x l -> A_predicate x) by intuition. specialize (IHl H5). clear H5.
       assert (length l <= fuel' /\ (forall x : A, In x l -> x <> A_halt)). split. apply le_S_n. intuition.
@@ -198,22 +202,4 @@ Section SteppingListCacheEncoder.
   Qed.
 End SteppingListCacheEncoder.
 
-Global Instance SteppingListCache_decoder A B fuel cache cacheAdd cacheGet cachePeek transformer
-       (A_halt : A)
-       (A_halt_dec : forall a, {a = A_halt} + {~ a = A_halt})
-       (A_predicate : A -> Prop)
-       (A_encode : A -> CacheEncode -> bin * CacheEncode)
-       (A_decoder : decoder cache transformer A_predicate A_encode)
-       (B_predicate : B -> Prop)
-       (B_encode : B -> CacheEncode -> bin * CacheEncode)
-       (B_decoder : decoder cache transformer B_predicate B_encode)
-       (C_predicate : CacheBranch -> Prop)
-       (C_encode : CacheBranch -> CacheEncode -> bin * CacheEncode)
-       (C_decoder : decoder cache transformer C_predicate C_encode)
-  : decoder cache transformer
-            (SteppingList_predicate A_predicate B_predicate C_predicate)
-            (SteppingList_encode cacheAdd cacheGet cachePeek transformer A_encode B_encode C_encode) :=
-  { decode := SteppingList_decode fuel cacheAdd cacheGet cachePeek A_halt_dec A_decoder B_decoder C_decoder;
-    decode_correct := @SteppingList_encode_correct _ _ _ _ _ _ _ _ _ _ _ _ _ _ _ _ _ _ _ }.
-
-Arguments SteppingList_encode {_ _ _ _ _ _ _} _ {_} _ _ _ _ _.
+Arguments SteppingList_encode {_ _ _ _ _ _ _ _ _ _} _ _ _ _ _.
